src/syntax/subst.fsi
@@ -42,6 +42,10 @@ val open_comp:          binders -> comp -> binders * comp
 val open_branch:        branch -> branch
 val open_let_rec:       list<letbinding> -> term -> list<letbinding> * term
 val open_univ_vars:     univ_names -> term -> univ_names * term
+val open_univ_vars_comp:univ_names -> comp -> univ_names * comp
 
 val subst_binders:      binders -> args -> term -> term
 val subst_binders_comp: binders -> args -> comp -> comp
+
+val close_tscheme: binders -> tscheme -> tscheme
+val close_univ_vars_tscheme: univ_names -> tscheme -> tscheme
